1-2

| p    | q    | ~p   | (~pVq) | ~q   | (p∧~q) | (~p∧q)V(p∧~q) |
| ---- | ---- | ---- | ------ | ---- | ------ | ------------- |
| T    | T    | F    | T      | F    | F      | T             |
| T    | F    | F    | F      | T    | T      | T             |
| F    | T    | T    | T      | F    | F      | T             |
| F    | F    | T    | T      | T    | F      | T             |

2-2

| p    | q    | (p∧q) | ~q   | (p∧~q) | (p∧q)∧(p∧~q) |
| ---- | ---- | ----- | ---- | ------ | ------------ |
| T    | T    | F     | F    | F      | F            |
| T    | F    | F     | T    | T      | F            |
| F    | T    | T     | F    | F      | F            |
| F    | F    | F     | T    | F      | F            |

3-2

| p    | q    | ~p   | ~q   | ~p∧~q | ~(pVq) |
| ---- | ---- | ---- | ---- | ----- | ------ |
| T    | T    | F    | F    | F     | F      |
| T    | F    | F    | T    | F     | F      |
| F    | T    | T    | F    | F     | F      |
| F    | F    | T    | T    | T     | T      |

4-2

~p∧~q

5-2

참

5-4

거짓

7

n=2m+1

n^2 = 4m^2 + 4m + 1

n^2 + n = 4m^2 + 6m + 2 = 2(2m^2 + 3m + 1)

9번

n=2m+1

n^2 = 4m^2 + 4m + 1

n^2+5 = n^2 = 4m^2 + 4m + 6 = 2(2m^2 + 2m + 3)

10번

n=2m+1 -> n^2 = 4m^2 + 4m + 1

따라서 n^2 짝수 -> n 짝수

11번

n=2m+1 

n^2 + 5n + 3 =  4m^2 + 14m + 9 = 2(2m^2 + 7m + 4) + 1 홀수

n = 2m

n^2 + 5n + 3 = 4m^2 + 10m + 3 = 2(2m^2 + 5m + 1) + 1 홀수

12번

n % 3 != 0 -> n^2 % 3 != 0

따라서 n^2 % 3 = 0 -> n % 3 = 0